SML with jumps (JSML) implemented; needs proving.

sml.v
@@ -5,51 +5,9 @@ Import ListNotations.
 
 Load utils.
 Load lambda.
+Load stack.
 
 Module SML.
-
-  (* TODO: stack_equiv showing empty and singleton tuples can be reduced *)
-  Inductive Stack: Set :=
-  | snil
-  | snat (n: nat) (s: Stack)
-  | stuple (t: Stack) (s: Stack).
-
-  Function stack_prefix (n: nat) (s: Stack): option Stack :=
-    match n with
-    | 0 => Some snil
-    | S n' =>
-      match s with
-      | snil => None
-      | snat m s =>
-        match stack_prefix n' s with
-        | None => None
-        | Some s' => Some (snat m s')
-        end
-      | stuple t s =>
-        match stack_prefix n' s with
-        | None => None
-        | Some s' => Some (stuple t s')
-        end
-      end
-    end.
-
-  Function stack_postfix (n: nat) (s: Stack): option Stack :=
-    match n with
-    | 0 => Some s
-    | S n' =>
-      match s with
-      | snil => None
-      | snat _ s'
-      | stuple _ s' => stack_postfix n' s'
-      end
-    end.
-
-  Function stack_append (s1 s2: Stack): Stack :=
-    match s1 with
-    | snil => s2
-    | snat n s => snat n (stack_append s s2)
-    | stuple t s => stuple t (stack_append s s2)
-    end.
 
   Inductive SMCommand : Set :=
   | push (n: nat)
@@ -62,93 +20,17 @@ Module SML.
   | out.
 
   Definition SMProgram := list SMCommand.
-
-  Inductive SMState :=
-    | running (smp: SMProgram)
-          (returns: list SMProgram)
-          (fn_table: list SMProgram)
-          (stack: Stack)
-          (output: list nat)
-    | halted (output: list nat)
-    | error.
-
-  Function stack_del (n: nat) (s: Stack): option Stack :=
-    match (s, n) with
-    | (snil, _) => None
-    | (snat _ s, 0)
-    | (stuple _ s, 0) => Some s
-    | (snat m s, S n) =>
-      match stack_del n s with
-      | None => None
-      | Some s' => Some (snat m s')
-      end
-    | (stuple t s, S n) =>
-      match stack_del n s with
-      | None => None
-      | Some s' => Some (stuple t s')
-      end
-    end.
-
-  Function stack_get (n: nat) (s: Stack): option Stack :=
-    match stack_postfix n s with
-    | None | Some snil => None
-    | Some (snat m _) => Some (snat m s)
-    | Some (stuple t _) => Some (stuple t s)
-    end.
-
-  Example stack_prefix_ex:
-    forall s, stack_prefix 1 (snat 3 s) = Some (snat 3 snil).
-  Proof. intros; auto. Qed.
-
-  Function stack_pack (n: nat) (s: Stack): option Stack :=
-    match n with
-    | 0 | 1 => Some s
-    | _ =>
-      match (stack_prefix n s, stack_postfix n s) with
-      | (Some t, Some s') => Some (stuple t s')
-      | _ => None
-      end
-    end.
-
-  Example stack_pack_simple:
-    stack_pack 2 (snat 0 (snat 1 snil)) =
-    Some (stuple (snat 0 (snat 1 snil)) snil).
-  Proof. auto. Qed.
-
-  Example stack_pack_nested:
-    forall tl,
-      stack_pack 3 (snat 1
-                         (stuple (snat 2 (snat 3 snil))
-                                 (snat 4 tl))) =
-      Some (stuple (snat 1
-                         (stuple (snat 2 (snat 3 snil))
-                                 (snat 4 snil)))
-                   tl).
-  Proof. intros; auto. Qed.
-
-  Function stack_unpack (s: Stack): option Stack :=
-    match s with
-    | snil => None
-    | snat _ _ => Some s
-    | stuple t s => Some (stack_append t s)
-    end.
-
-  Function stack_weight (s: Stack): nat :=
-    match s with
-    | snil => 0
-    | snat _ s' => S (stack_weight s')
-    | stuple t s' => S (stack_weight t + stack_weight s')
-    end.
+  Definition Stack := Stack.Stack.
 
   Function stack_call (s: Stack) (fn_table: list SMProgram)
-           {measure stack_weight s}: (option Stack) * SMProgram :=
-    match stack_unpack s with
+           {measure Stack.stack_weight s}: (option Stack) * SMProgram  :=
+    match Stack.stack_unpack s with
     | None => (None, [])
     | Some stack =>
       match stack with
-      | snil => (None, [])
-      | stuple t s' => stack_call stack fn_table
-      | snat fid s' =>
+      | Stack.snil => (None, [])
+      | Stack.stuple t s' => stack_call stack fn_table
+      | Stack.snat fid s' =>
         match nth_error fn_table fid with
         | None => (None, [])
         | Some fn => (Some s', fn)
@@ -158,23 +40,20 @@ Module SML.
   Proof.
     intros.
     destruct s; simpl in *; try discriminate.
-    assert (stack_append s1 s2 = stuple t s') by congruence.
+    assert (Stack.stack_append s1 s2 = Stack.stuple t s') by congruence.
     functional inversion H; subst; simpl in *; try omega.
     clear H teq.
     induction s; simpl in *; try omega.
   Defined.
 
-  Function stack_inc (s: Stack): option Stack :=
-    match s with
-    | snat m s' => Some (snat (S m) s')
-    | _ => None
-    end.
-
-  Function stack_out (s: Stack): (option nat) :=
-    match s with
-    | snat m s' => Some m
-    | _ => None
-    end.
+  Inductive SMState :=
+    | running (smp: SMProgram)
+          (returns: list SMProgram)
+          (fn_table: list SMProgram)
+          (stack: Stack)
+          (output: list nat)
+    | halted (output: list nat)
+    | error.
 
   Definition sm_step (s: SMState): SMState :=
     match s with
@@ -187,24 +66,24 @@ Module SML.
         | _ => halted output
         end
       | push n :: smp' =>
-        running smp' rets fn_table (snat n stack) output
+        running smp' rets fn_table (Stack.snat n stack) output
       | del n :: smp' =>
-        match stack_del n stack with
+        match Stack.stack_del n stack with
         | Some stack' => running smp' rets fn_table stack' output
         | None => error
         end
       | get n :: smp' =>
-        match stack_get n stack with
+        match Stack.stack_get n stack with
         | Some stack' => running smp' rets fn_table stack' output
         | None => error
         end
       | pack n :: smp' =>
-        match stack_pack n stack with
+        match Stack.stack_pack n stack with
         | Some stack' => running smp' rets fn_table stack' output
         | None => error
         end
       | unpack :: smp' =>
-        match stack_unpack stack with
+        match Stack.stack_unpack stack with
         | Some stack' => running smp' rets fn_table stack' output
         | None => error
         end
@@ -215,12 +94,12 @@ Module SML.
         | (None, _) => error
         end
       | inc :: smp' =>
-        match stack_inc stack with
+        match Stack.stack_inc stack with
         | Some stack' => running smp' rets fn_table stack' output
         | None => error
         end
       | out :: smp' =>
-        match stack_out stack with
+        match Stack.stack_out stack with
         | Some a => running smp' rets fn_table stack (output ++ [a])
         | None => error
         end
@@ -228,9 +107,9 @@ Module SML.
     end.
 
   Definition exec_init (main: SMProgram) (fn_table: list SMProgram) : SMState :=
-    running main [] fn_table snil [].
+    running main [] fn_table Stack.snil [].
 
-  Definition interpret (prog: SMProgram * list SMProgram) (fuel: nat):
+  Definition interpret_sm (prog: SMProgram * list SMProgram) (fuel: nat):
     option (list nat) :=
     let (main, fn_table) := prog in
     match Utils.run sm_step (exec_init main fn_table) fuel with
@@ -239,11 +118,11 @@ Module SML.
     end.
 
   Example push_simple:
-    interpret ([push 3; out], []) 20 = Some [3].
+    interpret_sm ([push 3; out], []) 20 = Some [3].
   Proof. auto. Qed.
 
   Example call_simple:
-    interpret ([push 0; out; call; push 2; out], [[push 3; out]]) 9 = Some [0; 3; 2].
+    interpret_sm ([push 0; out; call; push 2; out], [[push 3; out]]) 9 = Some [0; 3; 2].
   Proof. auto. Qed.
 
   Inductive Ctx :=
@@ -291,14 +170,14 @@ Module SML.
 
     Example run_trans_out_2:
     match (Lambda.parse_lambda "^(\f.\x.f (f x))") with
-    | Some l => interpret (sml_of_lambda l) 27
+    | Some l => interpret_sm (sml_of_lambda l) 27
     | None => None
     end = Some [2].
   Proof. auto. Qed.
 
   Example run_trans_out_f_id_2:
     match (Lambda.parse_lambda "^((\x.\y.y) (\x.x) (\f.\x.f (f x)))") with
-    | Some l => interpret (sml_of_lambda l) 42
+    | Some l => interpret_sm (sml_of_lambda l) 42
     | None => None
     end = Some [2].
   Proof. auto. Qed.
