jsml.v
@@ -1,0 +1,199 @@
+Require Import Arith.
+Require Import Omega.
+Require Import Coq.Lists.List.
+Import ListNotations.
+
+Load sml.
+
+Module JSML.
+  Inductive JSMCommand : Set :=
+  | push (n: nat)
+  | del (n: nat)
+  | get (n: nat)
+  | pack (n: nat)
+  | unpack
+
+  | inc
+  | out.
+
+  Definition JSMProgram := list JSMCommand.
+  Definition Stack := Stack.Stack.
+
+  Inductive JSMState :=
+    | running (smp: JSMProgram)
+          (fn_table: list JSMProgram)
+          (stack: Stack)
+          (output: list nat)
+    | halted (output: list nat)
+    | error.
+
+  Function stack_jump (s : Stack) (fn_table : list JSMProgram) 
+           {measure Stack.stack_weight s} :=
+    match Stack.stack_unpack s with
+    | None => (None, [])
+    | Some stack =>
+      match stack with
+      | Stack.snil => (None, [])
+      | Stack.stuple t s' => stack_jump stack fn_table
+      | Stack.snat fid s' =>
+        match nth_error fn_table fid with
+        | None => (None, [])
+        | Some fn => (Some s', fn)
+        end
+      end
+    end.
+   Proof.
+    intros.
+    destruct s; simpl in *; try discriminate.
+    assert (Stack.stack_append s1 s2 = Stack.stuple t s') by congruence.
+    functional inversion H; subst; simpl in *; try omega.
+    clear H teq.
+    induction s; simpl in *; try omega.
+  Defined.
+
+  Function jsm_step (s: JSMState): JSMState :=
+    match s with
+    | halted _ | error => s
+    | running smp fn_table stack output =>
+      match smp with
+      | [] =>
+        match stack_jump stack fn_table with
+        | (Some stack', smf) =>
+          running smf fn_table stack' output
+        | (None, _) => halted output
+        end
+      | push n :: smp' =>
+        running smp' fn_table (Stack.snat n stack) output
+      | del n :: smp' =>
+        match Stack.stack_del n stack with
+        | Some stack' => running smp' fn_table stack' output
+        | None => error
+        end
+      | get n :: smp' =>
+        match Stack.stack_get n stack with
+        | Some stack' => running smp' fn_table stack' output
+        | None => error
+        end
+      | pack n :: smp' =>
+        match Stack.stack_pack n stack with
+        | Some stack' => running smp' fn_table stack' output
+        | None => error
+        end
+      | unpack :: smp' =>
+        match Stack.stack_unpack stack with
+        | Some stack' => running smp' fn_table stack' output
+        | None => error
+        end
+      | inc :: smp' =>
+        match Stack.stack_inc stack with
+        | Some stack' => running smp' fn_table stack' output
+        | None => error
+        end
+      | out :: smp' =>
+        match Stack.stack_out stack with
+        | Some a => running smp' fn_table stack (output ++ [a])
+        | None => error
+        end
+      end
+    end.
+
+  Definition exec_init (main: JSMProgram) (fn_table: list JSMProgram) : JSMState :=
+    running main fn_table Stack.snil [].
+
+  Definition interpret_jsm (prog: JSMProgram * list JSMProgram) (fuel: nat):
+    option (list nat) :=
+    let (main, fn_table) := prog in
+    match Utils.run jsm_step (exec_init main fn_table) fuel with
+    | halted output => Some output
+    | _ => None
+    end.
+
+  Function jsmp_of_smp (smp : SML.SMProgram) (len : nat) (calls : list JSMProgram) : (JSMProgram * list JSMProgram) :=
+    match smp with
+    | SML.push n :: smp' =>
+      match jsmp_of_smp smp' len calls with
+      | (jsmp, calls) => (push n :: jsmp, calls)
+      end
+    | SML.get n :: smp' =>
+      match jsmp_of_smp smp' len calls with
+      | (jsmp, calls) => (get n :: jsmp, calls)
+      end
+    | SML.pack n :: smp' =>
+      match jsmp_of_smp smp' len calls with
+      | (jsmp, calls) => (pack n :: jsmp, calls)
+      end
+    | SML.del n :: smp' =>
+      match jsmp_of_smp smp' len calls with
+      | (jsmp, calls) => (del n :: jsmp, calls)
+      end
+    | SML.unpack :: smp' =>
+      match jsmp_of_smp smp' len calls with
+      | (jsmp, calls) => (unpack :: jsmp, calls)
+      end
+    | SML.out :: smp' =>
+      match jsmp_of_smp smp' len calls with
+      | (jsmp, calls) => (out :: jsmp, calls)
+      end
+    | SML.inc :: smp' =>
+      match jsmp_of_smp smp' len calls with
+      | (jsmp, calls) => (inc :: jsmp, calls)
+      end
+    | SML.call :: smp' =>
+      match jsmp_of_smp smp' len calls with
+      | (jsmp, calls) => ([push (len + List.length calls); get 1; del 2], calls ++ [jsmp])
+      end
+    | [] => ([], calls)
+  end.
+
+  Function jsm_of_sm' (fn_table : list SML.SMProgram) (start : list JSMProgram) 
+           (calls : list JSMProgram) (n : nat) : (list JSMProgram) :=
+    match fn_table with
+    | [] => start ++ calls
+    | smp :: tl =>
+       match jsmp_of_smp smp n calls with
+       | (jsmp, calls') => jsm_of_sm' tl (start ++ [jsmp]) calls' n
+       end
+    end.
+    
+  Function jsm_of_sm (sm : SML.SMProgram * list SML.SMProgram) : (JSMProgram * list JSMProgram) :=
+    match sm with
+    | (main, fn_table) =>
+      match jsmp_of_smp main (List.length fn_table) [] with
+      | (main', calls') => 
+          (main', jsm_of_sm' fn_table [] calls' (List.length fn_table))
+      end
+    end.
+
+  Theorem jsml_of_sml_correct :
+  forall (sm : SML.SMProgram * list SML.SMProgram) (input output: list nat),
+      (exists fuel, SML.interpret_sm sm fuel = Some output) ->
+      (exists fuel, interpret_jsm (jsm_of_sm sm) fuel = Some output).
+  Proof.
+    intros.
+    destruct H as [fuel]; exists fuel.
+    rewrite <- H; clear H.
+    unfold interpret_jsm, SML.interpret_sm.
+    (* finish proof... *)
+  Admitted.
+  
+  
+  (* NOT USEFUL: I was doing the wrong direction. Keeping it here just because...
+  Function smp_of_jsmp (jsmp : JSMProgram) : SML.SMProgram :=
+    match jsmp with
+    | push n :: jsmp' => SML.push n :: (smp_of_jsmp jsmp')
+    | del n :: jsmp' => SML.del n :: (smp_of_jsmp jsmp')
+    | get n :: jsmp' => SML.get n :: (smp_of_jsmp jsmp')
+    | pack n :: jsmp' => SML.pack n :: (smp_of_jsmp jsmp')
+    | unpack :: jsmp' => SML.unpack :: (smp_of_jsmp jsmp')
+    | out :: jsmp' => SML.out :: (smp_of_jsmp jsmp')
+    | inc :: jsmp' => SML.inc :: (smp_of_jsmp jsmp')
+    | [] => [SML.call]
+    end.
+
+  Function sm_of_jsm (jsmp : JSMProgram * list JSMProgram) : SML.SMProgram * list SML.SMProgram :=
+    match jsmp with
+    | (main, fn_table) => (smp_of_jsmp main, List.map smp_of_jsmp fn_table)
+    end.
+  *)
+
+End JSML.
